# CSE 280 Challenge Set 01

(c) BYU-Idaho 

## Question 1

Let the following statements by given:

* $a = $ "You used the pool in the afternoon."
* $b = $ "You cleaned up after lunch."
* $c = $ "You must clean up after dinner."

**Part 1**

Use connectives (operators) to translate the following statement into a compound proposition.

"If you used the pool in the afternoon and you didn't clean up after lunch, then you must clean up after dinner."

<br /><br />

**Part 2**

Construct a truth table for the compound proposition you found in Part 1.  The eight rows of your table should correspond to the eight different possibilities for $a$, $b$, and $c$.

|Row|$a$|$b$|$c$|$\neg b$|$a \land \neg b$|ANS|
|:-:|:-:|:-:|:-:|:-:|:-:|:-:|
|1|||||||
|2|||||||
|3|||||||
|4|||||||
|5|||||||
|6|||||||
|7|||||||
|8|||||||

**Part 3**

Suppose that the compound proposition given in part 1 is false.  What must be true about your pool usage and cleanup duties? 

## Question 2

Use a truth table to prove that the compound proposition $[(p \lor r) \land (\neg p)] \to r$ is always true or always false, no matter what $p$ and $r$ are.  What do we call this type of compound proposition?

<br /><br /><br /><br /><br />

## Question 3

Let $s$ be the following statement:  "If it's raining, then the ground is wet."

**Part 1**

Give the inverse of $s$.  Is this the same as $s$?

**Part 2**

Give the converse of $s$.  Is this the same as $s$?

**Part 3**

Give the contrapositive of $s$.  Is this the same as $s$?


## Question 4

Determine if the following propositions written in English are True or False:

* If 2 is even, then 5 is prime. 
* If 3 is even, then 6 is prime. 
* If 5 is odd, then 8 is prime. 
* If 8 is odd, then 11 is prime. 
* 10 is even if and only if 4 is prime 
* 11 is even if and only if 6 is prime 

## Question 5

Simplify the following using a truth table:

$\neg(A \to B) \lor \neg(A \lor B)$

<br /><br /><br /><br />

## Question 6

The following "ugly-looking" multi-line compound proposition is a Tautology.  Can you explain why without using a truth table.  Hint: Refer back to Question 3 above.

$((A \to B) \leftrightarrow (\neg B \to \neg A)) \land ((B \to A) \leftrightarrow (\neg A \to \neg B)) \land$

$((B \to C) \leftrightarrow (\neg C \to \neg B)) \land ((C \to B) \leftrightarrow (\neg B \to \neg C)) \land$

$((A \to C) \leftrightarrow (\neg C \to \neg A)) \land ((C \to A) \leftrightarrow (\neg A \to \neg C))$

